theories/Factor_Workflow_Execution_Sharing.thy
@@ -19,12 +19,13 @@ lemma evaluate_workflow_stage_source_shared_code [code]:
     | Some ys \<Rightarrow> (case finite_native_source (workflow_source S)
         (workflow_source_use S) (workflow_source_root S) of None \<Rightarrow> None
       | Some P \<Rightarrow> if workflow_entry S |\<notin>| finite_system_definitions P then None else
-        let D=finite_program_term_demand P (fset_of_list (map (Finite_Pair x) ys)) in
+        let D=finite_program_demanded_calls P (fset_of_list (map (Finite_Pair x) ys))
+          (fimage (Pair (workflow_entry S)) (fset_of_list (map (Finite_Pair x) ys))) in
         map_option (\<lambda>(A,T). (P,D,A,T,
           filter (\<lambda>y. (workflow_entry S,Finite_Pair x y) |\<in>| A) ys))
           (finite_program_proofs P D)))"
   by (auto simp: evaluate_workflow_stage_def workflow_scope_values_def workflow_stage_arguments_def
-    finite_native_program_proofs_def finite_source_computation_def Let_def option.map_comp comp_def
+    workflow_stage_demand_def workflow_stage_requests_def finite_native_program_proofs_def finite_source_computation_def Let_def option.map_comp comp_def
     split: option.splits prod.splits)
 
 declare workflow_stage_reference_def[code del]
@@ -34,11 +35,12 @@ lemma workflow_stage_reference_source_shared_code [code]:
     | Some ys \<Rightarrow> (case finite_native_source (workflow_source S)
         (workflow_source_use S) (workflow_source_root S) of None \<Rightarrow> None
       | Some P \<Rightarrow> if workflow_entry S |\<notin>| finite_system_definitions P then None else
-        let D=finite_program_term_demand P (fset_of_list (map (Finite_Pair x) ys)) in
+        let D=finite_program_demanded_calls P (fset_of_list (map (Finite_Pair x) ys))
+          (fimage (Pair (workflow_entry S)) (fset_of_list (map (Finite_Pair x) ys))) in
         map_option (\<lambda>A. filter (\<lambda>y. (workflow_entry S,Finite_Pair x y) |\<in>| A) ys)
           (finite_program_evaluation P D)))"
   by (auto simp: workflow_stage_reference_def workflow_scope_values_def workflow_stage_arguments_def
-    finite_native_program_evaluation_def finite_source_computation_def Let_def option.map_comp comp_def split: option.splits)
+    workflow_stage_demand_def workflow_stage_requests_def finite_native_program_evaluation_def finite_source_computation_def Let_def option.map_comp comp_def split: option.splits)
 
 declare workflow_stage_evidence_def[code del]
 
@@ -47,12 +49,13 @@ lemma workflow_stage_evidence_source_shared_code [code]:
     (case workflow_scope_result S input of None \<Rightarrow> False | Some scope \<Rightarrow>
       finite_native_source (workflow_source S) (workflow_source_use S) (workflow_source_root S)=Some P \<and>
       workflow_entry S |\<in>| finite_system_definitions P \<and>
-      D=finite_program_term_demand P (fset_of_list (map (Finite_Pair input) scope)) \<and>
+      D=finite_program_demanded_calls P (fset_of_list (map (Finite_Pair input) scope))
+        (fimage (Pair (workflow_entry S)) (fset_of_list (map (Finite_Pair input) scope))) \<and>
       finite_program_evaluation P D=Some A \<and>
       fimage fst T=A \<and> finite_inspection_rows_hold (finite_proof_inspection P T) \<and>
       ys=filter (\<lambda>y. (workflow_entry S,Finite_Pair input y) |\<in>| A) scope))"
   by (auto simp: workflow_stage_evidence_def workflow_scope_values_def workflow_stage_arguments_def
-    finite_native_program_evaluation_def finite_source_computation_def Let_def
+    workflow_stage_demand_def workflow_stage_requests_def finite_native_program_evaluation_def finite_source_computation_def Let_def
     split: option.splits prod.splits)
 
 text \<open>The actual complete scope and source are read once per stage.
